Finish br_ccopy fault tolerance proof

Examples/br_ccopy/br_ccopy_ft_proof.v
@@ -168,3 +168,147 @@ Proof using.
             now apply noverlap_symmetry.
     }
 Qed.
+
+Section FaultTolerantInvariants.
+    Variable ctl : N.
+    Variable dst src : addr.
+    Variable len : N.
+    Variable mem : memory.
+
+    Definition ft_invs T (Inv Post: inv_type T) (NoInv:T) (s:store) (a:addr) : T :=
+        match a with
+        | 0x0 => Inv 0 (
+                s R_A0 = ctl /\ s R_A1 = dst /\ s R_A2 = src /\ s R_A3 = len /\
+                s V_MEM32 = mem /\
+                ~ overlap 32 src len dst len /\
+                s V_FC = 1
+            )
+        | 0x20 => Inv 0 (exists k mem',
+                s V_MEM32 = mem' /\
+                s R_A0 = neg ctl /\
+                s R_A1 = dst ⊕ k /\
+                s R_A2 = src ⊕ k /\
+                s R_A6 = dst ⊕ len /\
+                k < len < 2^32 /\
+                ~ overlap 32 src len dst len /\
+                (ctl = 1 -> k_equal mem' src dst k) /\
+                s V_FC <= 1
+            )
+        | 0x90 | 0x94 => Post 0 (postcondition ctl dst src len s)
+        | _ => NoInv
+        end.
+
+    Definition br_ccopy_fault : program := inject_fault br_ccopy.
+
+    Definition ft_exits0 := make_exits 0 br_ccopy_fault ft_invs.
+    Definition ft_invs0 := make_invs 0 br_ccopy_fault ft_invs.
+End FaultTolerantInvariants.
+
+(* Proof in single-fault context *)
+Theorem br_ccopy_ft_correctness:
+  forall s mem t xs' ctl src dst len
+         (ENTRY: startof t xs' = (Addr 0, s))
+         (MDL: models rvtypctx s)
+         (MEM: s V_MEM32 = mem)
+         (A0: s R_A0 = ctl)
+         (A1: s R_A1 = dst)
+         (A2: s R_A2 = src)
+         (LEN: s R_A3 = len)
+         (NOV: ~ overlap 32 src len dst len)
+         (FC: s V_FC = 1),
+  satisfies_all br_ccopy_fault (ft_invs0 ctl dst src len mem)
+                               (ft_exits0 ctl dst src len mem) (xs'::t).
+Proof using.
+    Local Ltac step ::= 
+        match goal with
+        | [s' : store, FC : ?s' V_FC <= 1 |- _] =>
+            let H := fresh "H" in
+            assert (s' V_FC = 0 \/ s' V_FC = 1) as H by lia;
+            clear FC; destruct H
+        | _ => idtac
+        end;
+        time r5_step;
+        repeat match goal with
+        | [n : N, BC : ?n mod 2 = _ |- _] => clear BC n
+        | [s' : store, n : N, 
+            BC : (if 0 <? ?s' V_FC then ?n mod 2 else 0) = _ |- _] => clear BC n
+        | [H: ?x = ?x |- _] => clear H
+        end;
+        try discriminate.
+    intros. apply prove_invs.
+
+    simpl. rewrite ENTRY. step. repeat split; assumption.
+
+    intros.
+    eapply startof_prefix in ENTRY; try eassumption.
+    eapply preservation_exec_prog in MDL; try (eassumption || apply inject_fault_lift_riscv_welltyped).
+    clear - PRE MDL. rename t1 into t. rename s1 into s. rename a1 into a.
+
+    destruct_inv 32 PRE.
+
+    (* Intro *)
+    destruct PRE as (A0 & A1 & A2 & A3 & Mem & Nov & FC). {
+    repeat step.
+    all: match goal with
+        | [|- _ -> _] => intro; unfold k_equal; lia
+        | _ => exists 0; eexists; psimpl; repeat split; unfold k_equal; try lia;
+            [apply (models_var R_A3) in MDL; rewrite <- A3; apply MDL
+            |assumption]
+        end.
+    }
+
+    (* Loop *)
+    destruct PRE as (k & mem' & Mem & A0 & A1 & A2 & A6 & Bound & Nov & Eq & FC). {
+    Local Ltac solve_inv ctl dst src len k Eq :=
+        solve [exists (k + 1); eexists; psimpl; repeat split; try lia;
+        [assumption|];
+        intro; subst ctl; cbv [neg]; psimpl;
+        rewrite N.lxor_comm, <- N.lxor_assoc, N.lxor_nilpotent;
+        apply k_equal_step; unfold k_equal; intros; psimpl;
+        repeat rewrite getmem_noverlap;
+        match goal with
+        | [|- _ = _] => auto; now apply Eq
+        | [|- ~ overlap _ _ _ _ _] =>
+            (apply noverlap_single_lt; lia) ||
+            (apply (noverlap_shrink _ src len);
+            [psimpl; rewrite N.mod_small by lia; lia
+            |apply noverlap_symmetry, (noverlap_shrink _ dst len);
+                [psimpl; lia|now apply noverlap_symmetry]])
+        | _ => idtac
+        end].
+    Local Ltac solve_post ctl dst src len k Eq :=
+        solve [let i := fresh "i" in
+        let ILen := fresh "ILen" in
+        replace len with (k + 1) in * by lia;
+        intros; subst ctl; cbv [neg]; psimpl;
+        rewrite N.lxor_comm, <- N.lxor_assoc, N.lxor_nilpotent;
+        psimpl; apply k_equal_step;
+        [unfold k_equal; intros;
+        repeat rewrite getmem_noverlap; 
+        [symmetry;now apply Eq|
+        apply (noverlap_shrink _ src (k + 1));
+        [psimpl; lia|
+        apply noverlap_symmetry, (noverlap_shrink _ dst (k + 1));
+        [psimpl; lia|now apply noverlap_symmetry]]|
+        apply noverlap_single_lt; lia]
+        |psimpl;rewrite getmem_noverlap; auto;
+        apply (noverlap_shrink _ src (k + 1));
+        [psimpl; lia|
+        apply noverlap_symmetry, (noverlap_shrink _ dst (k + 1));
+        [psimpl; lia|now apply noverlap_symmetry]]]].
+    repeat (step;
+            (* Get to end of already-faulted branches *) 
+            lazymatch goal with
+            | [|- context[update _ V_FC 0]] => repeat step;
+                lazymatch goal with
+                | [|- exists _, _] => solve_inv ctl dst src len k Eq
+                | [|- _ -> _] => solve_post ctl dst src len k Eq
+                end
+            | [|- nextinv _ _ _ _ _] => idtac
+            end).
+    step. solve_inv ctl dst src len k Eq.
+    step; solve_post ctl dst src len k Eq.
+    step. solve_inv ctl dst src len k Eq.
+    solve_post ctl dst src len k Eq.
+    }
+Qed.
