Examples/crypto_memcmp/crypto_memcmp_proof.v
@@ -148,15 +148,6 @@ Proof using.
     }
 Qed.
 
-Definition inject_fault (p : program) (s : store) (a : addr) :=
-  match p s a with
-  | None => None
-  | Some (sz,q) => Some (sz,
-    If (BinOp OP_AND (BinOp OP_LT (Word 0x0 32) (Var V_FC)) (Unknown 1))
-      (Move V_FC (BinOp OP_MINUS (Var V_FC) (Word 0x1 32)))
-      q)
-  end.
-
 Section FaultTolerantInvariants.
     Variable mem : memory.
     Variable in_a in_b : addr.
@@ -186,27 +177,6 @@ Section FaultTolerantInvariants.
     Definition ft_exits0 := make_exits 0 fault_memcmp ft_invs.
     Definition ft_invs0 := make_invs 0 fault_memcmp ft_invs.
 End FaultTolerantInvariants.
-
-Lemma inject_fault_lift_riscv_welltyped : forall p,
-    welltyped_prog rvtypctx (inject_fault (lift_riscv p)).
-Proof.
-    intros p s a. unfold inject_fault, lift_riscv.
-    exists rvtypctx.
-    econstructor.
-    change 1 with (widthof_binop OP_AND 1). constructor.
-        change 1 with (widthof_binop OP_LT 32). constructor.
-        constructor. lia. constructor. reflexivity.
-        constructor.
-    econstructor. now right.
-        change 32 with (widthof_binop OP_MINUS 32). constructor.
-        now constructor.
-        constructor. lia.
-        eapply typchk_stmt_mono with (c := rvtypctx) (c0 := rvtypctx)
-            (q := Move V_FC (BinOp OP_MINUS (Var V_FC) (Word 1 32))).
-        reflexivity. reflexivity.
-    apply welltyped_rv2il.
-    reflexivity.
-Qed.
     
 (* Proof in fault-free context *)
 Theorem crypto_memcmp_ft_correctness:
